Proof of completeness 👌 (removed useless run consistency check)

Operational.thy
@@ -12,87 +12,87 @@ abbreviation uncurry_conf
 
 inductive operational_semantics_step :: "config \<Rightarrow> config \<Rightarrow> bool" ("_ \<hookrightarrow> _" 70) where
   instant_i:
-  "consistent_run \<Gamma> \<Longrightarrow>
+  "(* consistent_run \<Gamma> \<Longrightarrow> *)
    \<Gamma>, n \<turnstile> [] \<triangleright> \<Phi>
      \<hookrightarrow>  \<Gamma>, Suc n \<turnstile> \<Phi> \<triangleright> []"
 | sporadic_e1:
-  "consistent_run \<Gamma> \<Longrightarrow>
+  "(* consistent_run \<Gamma> \<Longrightarrow> *)
    \<Gamma>, n \<turnstile> (K sporadic \<tau>) # \<Psi> \<triangleright> \<Phi>
      \<hookrightarrow>  \<Gamma>, n \<turnstile> \<Psi> \<triangleright> (K sporadic \<tau>) # \<Phi>"
 | sporadic_e2:
-  "consistent_run ((K \<Up> n) # (K \<Down> n @ \<lfloor>\<tau>\<rfloor>) # \<Gamma>) \<Longrightarrow>
+  "(* consistent_run ((K \<Up> n) # (K \<Down> n @ \<lfloor>\<tau>\<rfloor>) # \<Gamma>) \<Longrightarrow> *)
    \<Gamma>, n \<turnstile> (K sporadic \<tau>) # \<Psi> \<triangleright> \<Phi>
      \<hookrightarrow>  K \<Up> n # K \<Down> n @ \<lfloor>\<tau>\<rfloor> # \<Gamma>, n \<turnstile> \<Psi> \<triangleright> \<Phi>"
 | sporadic_on_e1:
-  "consistent_run \<Gamma> \<Longrightarrow>
+  "(* consistent_run \<Gamma> \<Longrightarrow> *)
    \<Gamma>, n \<turnstile> (K\<^sub>1 sporadic \<tau> on K\<^sub>2) # \<Psi> \<triangleright> \<Phi>
      \<hookrightarrow>  \<Gamma>, n \<turnstile> \<Psi> \<triangleright> (K\<^sub>1 sporadic \<tau> on K\<^sub>2) # \<Phi>"
 | sporadic_on_e2:
-  "consistent_run ((K\<^sub>1 \<Up> n) # (K\<^sub>2 \<Down> n @ \<tau>) # \<Gamma>) \<Longrightarrow>
+  "(* consistent_run ((K\<^sub>1 \<Up> n) # (K\<^sub>2 \<Down> n @ \<tau>) # \<Gamma>) \<Longrightarrow> *)
    \<Gamma>, n \<turnstile> (K\<^sub>1 sporadic \<tau> on K\<^sub>2) # \<Psi> \<triangleright> \<Phi>
      \<hookrightarrow>  K\<^sub>1 \<Up> n # K\<^sub>2 \<Down> n @ \<tau> # \<Gamma>, n \<turnstile> \<Psi> \<triangleright> \<Phi>"
 | tagrel_e:
-  "consistent_run ((\<tau>\<^sub>v\<^sub>a\<^sub>r(K\<^sub>1, n) \<doteq> \<alpha> * \<tau>\<^sub>v\<^sub>a\<^sub>r(K\<^sub>2, n) + \<beta>) # \<Gamma>) \<Longrightarrow>
+  "(* consistent_run ((\<tau>\<^sub>v\<^sub>a\<^sub>r(K\<^sub>1, n) \<doteq> \<alpha> * \<tau>\<^sub>v\<^sub>a\<^sub>r(K\<^sub>2, n) + \<beta>) # \<Gamma>) \<Longrightarrow> *)
    \<Gamma>, n \<turnstile> (tag-relation K\<^sub>1 = \<alpha> * K\<^sub>2 + \<beta>) # \<Psi> \<triangleright> \<Phi>
      \<hookrightarrow>  (\<tau>\<^sub>v\<^sub>a\<^sub>r(K\<^sub>1, n) \<doteq> \<alpha> * \<tau>\<^sub>v\<^sub>a\<^sub>r(K\<^sub>2, n) + \<beta>) # \<Gamma>, n \<turnstile> \<Psi> \<triangleright> (tag-relation K\<^sub>1 = \<alpha> * K\<^sub>2 + \<beta>) # \<Phi>"
 | implies_e1:
-  "consistent_run (K\<^sub>1 \<not>\<Up> n # \<Gamma>) \<Longrightarrow>
+  "(* consistent_run (K\<^sub>1 \<not>\<Up> n # \<Gamma>) \<Longrightarrow> *)
    \<Gamma>, n \<turnstile> (K\<^sub>1 implies K\<^sub>2) # \<Psi> \<triangleright> \<Phi>
      \<hookrightarrow>  K\<^sub>1 \<not>\<Up> n # \<Gamma>, n \<turnstile> \<Psi> \<triangleright> (K\<^sub>1 implies K\<^sub>2) # \<Phi>"
 | implies_e2:
-  "consistent_run ((K\<^sub>1 \<Up> n) # (K\<^sub>2 \<Up> n) # \<Gamma>) \<Longrightarrow>
+  "(* consistent_run ((K\<^sub>1 \<Up> n) # (K\<^sub>2 \<Up> n) # \<Gamma>) \<Longrightarrow> *)
    \<Gamma>, n \<turnstile> (K\<^sub>1 implies K\<^sub>2) # \<Psi> \<triangleright> \<Phi>
      \<hookrightarrow>  K\<^sub>1 \<Up> n # K\<^sub>2 \<Up> n # \<Gamma>, n \<turnstile> \<Psi> \<triangleright> (K\<^sub>1 implies K\<^sub>2) # \<Phi>"
 | timedelayed_e1:
-  "consistent_run (K\<^sub>1 \<not>\<Up> n # \<Gamma>) \<Longrightarrow>
+  "(* consistent_run (K\<^sub>1 \<not>\<Up> n # \<Gamma>) \<Longrightarrow> *)
    \<Gamma>, n \<turnstile> (K\<^sub>1 time-delayed by \<delta>\<tau> on K\<^sub>2 implies K\<^sub>3) # \<Psi> \<triangleright> \<Phi>
      \<hookrightarrow>  K\<^sub>1 \<not>\<Up> n # \<Gamma>, n \<turnstile> \<Psi> \<triangleright> (K\<^sub>1 time-delayed by \<delta>\<tau> on K\<^sub>2 implies K\<^sub>3) # \<Phi>"
 | timedelayed_e2:
-  "consistent_run (K\<^sub>1 \<Up> n # \<Gamma>) \<Longrightarrow>
+  "(* consistent_run (K\<^sub>1 \<Up> n # \<Gamma>) \<Longrightarrow> *)
    \<Gamma>, n \<turnstile> (K\<^sub>1 time-delayed by \<delta>\<tau> on K\<^sub>2 implies K\<^sub>3) # \<Psi> \<triangleright> \<Phi>
      \<hookrightarrow>  K\<^sub>1 \<Up> n # \<Gamma>, n \<turnstile> (K\<^sub>3 sporadic \<lfloor>\<tau>\<^sub>v\<^sub>a\<^sub>r(K\<^sub>2, n) \<oplus> \<delta>\<tau>\<rfloor> on K\<^sub>2) # \<Psi> \<triangleright> (K\<^sub>1 time-delayed by \<delta>\<tau> on K\<^sub>2 implies K\<^sub>3) # \<Phi>"
 
 inductive operational_semantics_intro :: "config \<Rightarrow> config \<Rightarrow> bool" ("_ \<hookrightarrow>\<^sub>i _" 70) where
   instant_i:
-  "consistent_run \<Gamma> \<Longrightarrow>
+  "(* consistent_run \<Gamma> \<Longrightarrow> *)
    \<Gamma>, n \<turnstile> [] \<triangleright> \<Phi>
      \<hookrightarrow>\<^sub>i  \<Gamma>, Suc n \<turnstile> \<Phi> \<triangleright> []"
 
 inductive operational_semantics_elim :: "config \<Rightarrow> config \<Rightarrow> bool" ("_ \<hookrightarrow>\<^sub>e _" 70) where
   sporadic_e1:
-  "consistent_run \<Gamma> \<Longrightarrow>
+  "(* consistent_run \<Gamma> \<Longrightarrow> *)
    \<Gamma>, n \<turnstile> (K sporadic \<tau>) # \<Psi> \<triangleright> \<Phi>
      \<hookrightarrow>\<^sub>e  \<Gamma>, n \<turnstile> \<Psi> \<triangleright> (K sporadic \<tau>) # \<Phi>"
 | sporadic_e2:
-  "consistent_run ((K \<Up> n) # (K \<Down> n @ \<lfloor>\<tau>\<rfloor>) # \<Gamma>) \<Longrightarrow>
+  "(* consistent_run ((K \<Up> n) # (K \<Down> n @ \<lfloor>\<tau>\<rfloor>) # \<Gamma>) \<Longrightarrow> *)
    \<Gamma>, n \<turnstile> (K sporadic \<tau>) # \<Psi> \<triangleright> \<Phi>
      \<hookrightarrow>\<^sub>e  K \<Up> n # K \<Down> n @ \<lfloor>\<tau>\<rfloor> # \<Gamma>, n \<turnstile> \<Psi> \<triangleright> \<Phi>"
 | sporadic_on_e1:
-  "consistent_run \<Gamma> \<Longrightarrow>
+  "(* consistent_run \<Gamma> \<Longrightarrow> *)
    \<Gamma>, n \<turnstile> (K\<^sub>1 sporadic \<tau> on K\<^sub>2) # \<Psi> \<triangleright> \<Phi>
      \<hookrightarrow>\<^sub>e  \<Gamma>, n \<turnstile> \<Psi> \<triangleright> (K\<^sub>1 sporadic \<tau> on K\<^sub>2) # \<Phi>"
 | sporadic_on_e2:
-  "consistent_run ((K\<^sub>1 \<Up> n) # (K\<^sub>2 \<Down> n @ \<tau>) # \<Gamma>) \<Longrightarrow>
+  "(* consistent_run ((K\<^sub>1 \<Up> n) # (K\<^sub>2 \<Down> n @ \<tau>) # \<Gamma>) \<Longrightarrow> *)
    \<Gamma>, n \<turnstile> (K\<^sub>1 sporadic \<tau> on K\<^sub>2) # \<Psi> \<triangleright> \<Phi>
      \<hookrightarrow>\<^sub>e  K\<^sub>1 \<Up> n # K\<^sub>2 \<Down> n @ \<tau> # \<Gamma>, n \<turnstile> \<Psi> \<triangleright> \<Phi>"
 | tagrel_e:
-  "consistent_run ((\<tau>\<^sub>v\<^sub>a\<^sub>r(K\<^sub>1, n) \<doteq> \<alpha> * \<tau>\<^sub>v\<^sub>a\<^sub>r(K\<^sub>2, n) + \<beta>) # \<Gamma>) \<Longrightarrow>
+  "(* consistent_run ((\<tau>\<^sub>v\<^sub>a\<^sub>r(K\<^sub>1, n) \<doteq> \<alpha> * \<tau>\<^sub>v\<^sub>a\<^sub>r(K\<^sub>2, n) + \<beta>) # \<Gamma>) \<Longrightarrow> *)
    \<Gamma>, n \<turnstile> (tag-relation K\<^sub>1 = \<alpha> * K\<^sub>2 + \<beta>) # \<Psi> \<triangleright> \<Phi>
      \<hookrightarrow>\<^sub>e  (\<tau>\<^sub>v\<^sub>a\<^sub>r(K\<^sub>1, n) \<doteq> \<alpha> * \<tau>\<^sub>v\<^sub>a\<^sub>r(K\<^sub>2, n) + \<beta>) # \<Gamma>, n \<turnstile> \<Psi> \<triangleright> (tag-relation K\<^sub>1 = \<alpha> * K\<^sub>2 + \<beta>) # \<Phi>"
 | implies_e1:
-  "consistent_run (K\<^sub>1 \<not>\<Up> n # \<Gamma>) \<Longrightarrow>
+  "(* consistent_run (K\<^sub>1 \<not>\<Up> n # \<Gamma>) \<Longrightarrow> *)
    \<Gamma>, n \<turnstile> (K\<^sub>1 implies K\<^sub>2) # \<Psi> \<triangleright> \<Phi>
      \<hookrightarrow>\<^sub>e  K\<^sub>1 \<not>\<Up> n # \<Gamma>, n \<turnstile> \<Psi> \<triangleright> (K\<^sub>1 implies K\<^sub>2) # \<Phi>"
 | implies_e2:
-  "consistent_run ((K\<^sub>1 \<Up> n) # (K\<^sub>2 \<Up> n) # \<Gamma>) \<Longrightarrow>
+  "(* consistent_run ((K\<^sub>1 \<Up> n) # (K\<^sub>2 \<Up> n) # \<Gamma>) \<Longrightarrow> *)
    \<Gamma>, n \<turnstile> (K\<^sub>1 implies K\<^sub>2) # \<Psi> \<triangleright> \<Phi>
      \<hookrightarrow>\<^sub>e  K\<^sub>1 \<Up> n # K\<^sub>2 \<Up> n # \<Gamma>, n \<turnstile> \<Psi> \<triangleright> (K\<^sub>1 implies K\<^sub>2) # \<Phi>"
 | timedelayed_e1:
-  "consistent_run (K\<^sub>1 \<not>\<Up> n # \<Gamma>) \<Longrightarrow>
+  "(* consistent_run (K\<^sub>1 \<not>\<Up> n # \<Gamma>) \<Longrightarrow> *)
    \<Gamma>, n \<turnstile> (K\<^sub>1 time-delayed by \<delta>\<tau> on K\<^sub>2 implies K\<^sub>3) # \<Psi> \<triangleright> \<Phi>
      \<hookrightarrow>\<^sub>e  K\<^sub>1 \<not>\<Up> n # \<Gamma>, n \<turnstile> \<Psi> \<triangleright> (K\<^sub>1 time-delayed by \<delta>\<tau> on K\<^sub>2 implies K\<^sub>3) # \<Phi>"
 | timedelayed_e2:
-  "consistent_run (K\<^sub>1 \<Up> n # \<Gamma>) \<Longrightarrow>
+  "(* consistent_run (K\<^sub>1 \<Up> n # \<Gamma>) \<Longrightarrow> *)
    \<Gamma>, n \<turnstile> (K\<^sub>1 time-delayed by \<delta>\<tau> on K\<^sub>2 implies K\<^sub>3) # \<Psi> \<triangleright> \<Phi>
      \<hookrightarrow>\<^sub>e  K\<^sub>1 \<Up> n # \<Gamma>, n \<turnstile> (K\<^sub>3 sporadic \<lfloor>\<tau>\<^sub>v\<^sub>a\<^sub>r(K\<^sub>2, n) \<oplus> \<delta>\<tau>\<rfloor> on K\<^sub>2) # \<Psi> \<triangleright> (K\<^sub>1 time-delayed by \<delta>\<tau> on K\<^sub>2 implies K\<^sub>3) # \<Phi>"
 
